Revert "distinguished continuations." Going back to first class continuations.
This reverts commit 20e99e2ecd7b11b2ecc59ee38a0eb3bbb7973582.

src/AlphaEquivCps.v
@@ -15,14 +15,11 @@ Module Alpha.
   Section maps.
     Variable env_v : Type -> Type.
     Context {Mv : DMap var env_v}.
-    Variable env_cont : Type -> Type.
-    Context {Mcont : DMap cont env_cont}.
     
     Section monadic. 
       Variable m : Type -> Type.
       Context {Monad_m : Monad m}.
-      Context {Reader_vars : MonadReader (env_v var) m}.
-      Context {Reader_conts : MonadReader (env_cont cont) m}.
+      Context {Reader_m : MonadReader (env_v var) m}.
       Context {Zero_m : MonadZero m}.
 
       Import MonadNotation.
@@ -44,13 +41,6 @@ Module Alpha.
           | _ , _ => assert false
         end.
 
-      Definition alpha_cont (o1 o2 : cont) : m unit :=
-        x <- asks (lookup o1) ;;
-        match x with
-          | None => assert (eq_dec o1 o2)
-          | Some o => assert (eq_dec o o2)
-        end.
-
       Fixpoint all2 {T} (p : T -> T -> m unit) (ls1 ls2 : list T) : m unit :=
         match ls1 , ls2 with
           | nil , nil => ret tt
@@ -70,17 +60,12 @@ Module Alpha.
 
       Fixpoint alpha_exp' (e1 e2 : exp) {struct e1} : m unit :=
         match e1, e2 with
-          | App_e f1 k1 args1 , App_e f2 k2 args2 =>
+          | App_e f1 args1 , App_e f2 args2 =>
             alpha_op f1 f2 ;;
-            alpha_cont k1 k2 ;;
-            all2 alpha_op args1 args2
-          | AppK_e k1 args1 , AppK_e k2 args2 =>
-            alpha_cont k1 k2 ;;
             all2 alpha_op args1 args2
           | Let_e ds1 e1 , Let_e ds2 e2 =>
+            (** ignore permutations for now... **)
             alpha_dec ds1 ds2 (alpha_exp' e1 e2)
-          | Letrec_e ds1 e1 , Letrec_e ds2 e2 =>
-            assert false (** TODO **)
           | Switch_e op1 br1 e1 , Switch_e op2 br2 e2 =>
             alpha_op op1 op2 ;;
             match e1 , e2 with
@@ -114,7 +99,7 @@ Module Alpha.
             assert (eq_dec p1 p2) ;;
             all2 alpha_op args1 args2 ;;
             local (fun x => add v1 v2 (add w1 w2 x)) k
-          | Fn_d v1 k1 a1 e1 , Fn_d v2 k2 a2 e2 =>
+          | Fn_d v1 a1 e1 , Fn_d v2 a2 e2 =>
             (fix map_multi (x y : list var) (k : m unit) : m unit :=
               match x , y with
                 | nil , nil => k
@@ -122,24 +107,24 @@ Module Alpha.
                   local (add x y) (map_multi xs ys k)
                 | _ , _ => assert false
               end) a1 a2 (alpha_exp' e1 e2) ;;
-            local (add v1 v2) (local (add k1 k2) k) 
+            local (add v1 v2) k 
           | _ , _ => assert false
         end.
     End monadic.
   End maps.
 
   Definition alpha_exp (e1 e2 : exp) : bool :=
-    let res := runReader (runReaderT (unOptionT (alpha_exp' (m := optionT (readerT (alist cont cont) (reader (alist var var)))) e1 e2)) empty) empty in
+    let res := runReader (unOptionT (alpha_exp' (m := optionT (reader (alist var var))) e1 e2)) empty in
     match res with
       | None => false
       | Some _ => true
     end.
 
-  Definition alpha_k (e1 e2 : exp) : list var -> list var -> bool :=
+  Definition alpha_lam (e1 e2 : exp) : list var -> list var -> bool :=
     (fix build acc l1 l2 {struct l1} : bool :=
       match l1 , l2 with
         | nil , nil => 
-          let res := runReader (runReaderT (unOptionT (alpha_exp' (m := optionT (readerT (alist cont cont) (reader (alist var var)))) e1 e2)) empty) acc in
+          let res := runReader (unOptionT (alpha_exp' (m := optionT (reader (alist var var))) e1 e2)) acc in
           match res with
             | None => false
             | Some _ => true
@@ -148,21 +133,6 @@ Module Alpha.
           build (add l1 l2 acc) ls1 ls2
         | _ , _ => false
       end) empty.
-
-  Definition alpha_lam (e1 e2 : exp) (c1 c2 : cont) : list var -> list var -> bool :=
-    (fix build acc l1 l2 {struct l1} : bool :=
-      match l1 , l2 with
-        | nil , nil => 
-          let res := runReader (runReaderT (unOptionT (alpha_exp' (m := optionT (readerT (alist cont cont) (reader (alist var var)))) e1 e2)) (singleton c1 c2)) acc in
-          match res with
-            | None => false
-            | Some _ => true
-          end
-        | l1 :: ls1 , l2 :: ls2 =>
-          build (add l1 l2 acc) ls1 ls2
-        | _ , _ => false
-      end) empty.
-
   
   Module TEST.
     Require Import String.
@@ -176,10 +146,10 @@ Module Alpha.
     Goal (alpha_exp (f (wrapVar "0")) (f (wrapVar "0")) = true)%string.
     Proof. vm_compute; reflexivity. Abort.
 
-    Goal (alpha_k (f (wrapVar "0")) (f (wrapVar "1")) (wrapVar "0" :: nil) (wrapVar "1" :: nil) = true)%string.
+    Goal (alpha_lam (f (wrapVar "0")) (f (wrapVar "1")) (wrapVar "0" :: nil) (wrapVar "1" :: nil) = true)%string.
     Proof. vm_compute; reflexivity. Abort.
 
-    Goal (alpha_k (f (wrapVar "0")) (f (wrapVar "1")) (wrapVar "0" :: nil) (wrapVar "2" :: nil) = false)%string.
+    Goal (alpha_lam (f (wrapVar "0")) (f (wrapVar "1")) (wrapVar "0" :: nil) (wrapVar "2" :: nil) = false)%string.
     Proof. vm_compute; reflexivity. Abort.
 
   End TEST.
